\begin{align*}
    \sinh x = \frac{1}{2}(e^x - e^{-x}) &&& \cosh x = \frac{1}{2}(e^x + e^{-x}) \\
    \sin n\pi = 0 &&& \cos n\pi = (-1)^n
\end{align*}
\begin{align*}
\sin(\alpha+\beta)&{}=\sin \alpha\cos \beta+\cos \alpha\sin \beta\\
\cos(\alpha+\beta)&{}=\cos \alpha\cos \beta-\sin \alpha\sin \beta\\
\sin(2\alpha) &{}=2\cos \alpha \sin \alpha \\
\cos(2\alpha) &{}=\cos^2 \alpha - \sin^2 \alpha \\
         &{}=2\cos^2 \alpha - 1 \\
         &{}=1 - 2 \sin^2 \alpha
\end{align*}
\begin{align*}
\tan(\alpha+\beta)&{}=\dfrac{\tan \alpha+\tan \beta}{1-\tan \alpha\tan \beta}\\
\sin \alpha+\sin \beta&{}=2\sin\dfrac{\alpha+\beta}{2}\cos\dfrac{\alpha-\beta}{2}\\
\cos \alpha+\cos \beta&{}=2\cos\dfrac{\alpha+\beta}{2}\cos\dfrac{\alpha-\beta}{2} \\
\sin \alpha \sin \beta&{}=\frac{1}{2}(\cos(\alpha - \beta) - \cos(\alpha + \beta)) \\
\sin \alpha \cos \beta&{}=\frac{1}{2}(\sin(\alpha + \beta) + \sin(\alpha - \beta)) \\
\cos \alpha \sin \beta&{}=\frac{1}{2}(\sin(\alpha + \beta) - \sin(\alpha - \beta)) \\
\cos \alpha \cos \beta&{}=\frac{1}{2}(\cos(\alpha - \beta) + \cos(\alpha + \beta))
\end{align*}
\[ (V+W)\tan(\alpha-\beta)/2{}=(V-W)\tan(\alpha+\beta)/2 \]
where $V, W$ are lengths of sides opposite angles $\alpha, \beta$.
\begin{align*}
	a\cos x+b\sin x&=r\cos(x-\phi)\\
	a\sin x+b\cos x&=r\sin(x+\phi)
\end{align*}
where $r=\sqrt{a^2+b^2}, \phi=\operatorname{atan2}(b,a)$.
